RelationalAlgebra/FOL/WellTyped.lean
@@ -7,41 +7,41 @@ theorem Finset.empty.contra (s₁ : Finset Attribute) : (s₁ ≠ ∅) → (s₁
 
 namespace FOL
 
-def BoundedQuery.isWellTyped {n} : BoundedQuery n → Prop
-  | R _ _ _      => True
-  | tEq q t₁ t₂  => q.isWellTyped ∧ q.hasSafeTerm t₁ ∧ q.hasSafeTerm t₂
-  | and q₁ q₂    => q₁.isWellTyped ∧ q₂.isWellTyped
-  | ex q         => q.isWellTyped
+def BoundedQuery.isWellTyped {n} (dbs : DatabaseSchema) : BoundedQuery n → Prop
+  | R dbs' _ _   => dbs' = dbs
+  | tEq q t₁ t₂  => q.isWellTyped dbs ∧ q.hasSafeTerm t₁ ∧ q.hasSafeTerm t₂
+  | and q₁ q₂    => q₁.isWellTyped dbs ∧ q₂.isWellTyped dbs
+  | ex q         => q.isWellTyped dbs
 
 @[simp]
-theorem BoundedQuery.isWellTyped.R_def {dbs rn n} {f : Fin (Finset.card (dbs rn)) → fol.Term (Attribute ⊕ Fin n)} :
-  (R dbs rn f).isWellTyped := by simp [isWellTyped]
+theorem BoundedQuery.isWellTyped.R_def {dbs rn n} {f : Fin (Finset.card (dbs' rn)) → fol.Term (Attribute ⊕ Fin n)} :
+  (R dbs' rn f).isWellTyped dbs ↔ dbs' = dbs := by rfl
 
 @[simp]
 theorem BoundedQuery.isWellTyped.tEq_def {n} {q : BoundedQuery n} {t₁ t₂ : fol.Term (Attribute ⊕ Fin n)} :
-  (tEq q t₁ t₂).isWellTyped = (q.isWellTyped ∧ q.hasSafeTerm t₁ ∧ q.hasSafeTerm t₂) := rfl
+  (tEq q t₁ t₂).isWellTyped dbs = (q.isWellTyped dbs ∧ q.hasSafeTerm t₁ ∧ q.hasSafeTerm t₂) := rfl
 
 @[simp]
 theorem BoundedQuery.isWellTyped.and_def {n} {q₁ q₂ : BoundedQuery n} :
-  (and q₁ q₂).isWellTyped = (q₁.isWellTyped ∧ q₂.isWellTyped) := rfl
+  (and q₁ q₂).isWellTyped dbs = (q₁.isWellTyped dbs ∧ q₂.isWellTyped dbs) := rfl
 
 @[simp]
 theorem BoundedQuery.isWellTyped.ex_def {n} {q : BoundedQuery (n + 1)} :
-  (ex q).isWellTyped = q.isWellTyped := rfl
+  (ex q).isWellTyped dbs = q.isWellTyped dbs := rfl
 
 @[simp]
 theorem BoundedQuery.isWellTyped.exs_def {n} {q : BoundedQuery n} :
-  (exs q).isWellTyped = q.isWellTyped := by
+  (exs q).isWellTyped dbs = q.isWellTyped dbs := by
     induction n with
     | zero => simp_all only [exs_0]
     | succ n' ih => exact ih
 
 @[simp]
-theorem BoundedQuery.isWellTyped.and_comm {n} {q₁ q₂ : BoundedQuery n} (h : (and q₁ q₂).isWellTyped) :
-  (and q₂ q₁).isWellTyped
+theorem BoundedQuery.isWellTyped.and_comm {n} {q₁ q₂ : BoundedQuery n} (h : (and q₁ q₂).isWellTyped dbs) :
+  (and q₂ q₁).isWellTyped dbs
     := by simp_all [Finset.union_comm]
 
 @[simp]
-theorem BoundedQuery.isWellTyped.and_from_both {n} {q₁ q₂ : BoundedQuery n} (h₁ : q₁.isWellTyped) (h₂ : q₂.isWellTyped) :
-  (and q₁ q₂).isWellTyped
+theorem BoundedQuery.isWellTyped.and_from_both {n} {q₁ q₂ : BoundedQuery n} (h₁ : q₁.isWellTyped dbs) (h₂ : q₂.isWellTyped dbs) :
+  (and q₁ q₂).isWellTyped dbs
     := by simp_all only [and_def, and_self]
