RelationalAlgebra/Equivalence/Equivalence.lean
@@ -5,102 +5,95 @@ open RM
 @[simp]
 theorem ra_to_fol_evalT.FOL_evaluateT (dbi : DatabaseInstance) [struc : FOL.folStruc dbi] (raQ : RA.Query) :
   t ∈ (ra_to_fol_query raQ dbi.schema).evaluateT dbi ↔ (ra_to_fol_query raQ dbi.schema).RealizeDom dbi t := by
-    simp_all only [FOL.Query.evaluateT, FOL.Query.RealizeDom.def, FOL.BoundedQuery.RealizeDom.def,
-      FOL.BoundedQuery.RealizeValidDom.def, IsEmpty.forall_iff,
-      DatabaseInstance.default_ran_sub_domain, and_self, and_true, Set.mem_setOf_eq]
+    simp_all only [FOL.Query.evaluateT, FOL.Query.RealizeDom.def, Set.mem_setOf_eq]
 
 -- @TODO: Split this over multiple smaller proofs
-theorem ra_to_fol_evalT.reverse {raQ dbi} [struc : FOL.folStruc dbi] (h : RA.Query.isWellTyped dbi.schema raQ) :
+theorem ra_to_fol_evalT.fr {raQ dbi} [struc : FOL.folStruc dbi] (h : RA.Query.isWellTyped dbi.schema raQ) :
   ∀t, (ra_to_fol_query raQ dbi.schema).RealizeDom dbi t → t ∈ RA.Query.evaluateT dbi raQ := by
     induction raQ with
     | R rn =>
       intro t
       simp_all only [RA.Query.isWellTyped.R_def, ra_to_fol_query, FOL.Query.RealizeDom.def,
-        FOL.BoundedQuery.RealizeDom.def, FOL.BoundedQuery.Realize.R_def, Function.comp_apply,
-        FOL.outVar.def, FOL.Term.realizeSome.def, FirstOrder.Language.Term.realize_var,
-        Sum.elim_inl, FOL.BoundedQuery.toFormula_rel,
-        FirstOrder.Language.BoundedFormula.realize_rel, FOL.folStruc_apply_RelMap,
-        FOL.BoundedQuery.RealizeValidDom.def, FOL.BoundedQuery.schema.R_def,
+        FOL.BoundedQuery.Realize.R_def, Function.comp_apply, FOL.outVar.def,
+        FOL.Term.realizeSome.def, FirstOrder.Language.Term.realize_var, Sum.elim_inl,
+        FOL.BoundedQuery.toFormula_rel, FirstOrder.Language.BoundedFormula.realize_rel,
+        FOL.folStruc_apply_RelMap, FOL.BoundedQuery.schema.R_def,
         FirstOrder.Language.Term.varFinsetLeft.eq_1, Finset.mem_singleton,
-        RelationSchema.Dom_sub_fromIndex, Finset.toFinset_coe, IsEmpty.forall_iff,
-        DatabaseInstance.default_ran_sub_domain, and_self, and_true, RA.Query.evaluateT.R_def,
-        and_imp]
-      intro a a_1 a_2 a_3 a_4
-      simp_all only [RelationSchema.fromIndex_mem, implies_true]
+        RelationSchema.Dom_sub_fromIndex, Finset.toFinset_coe, RA.Query.evaluateT.R_def, and_imp]
+      intro a a_1 a_2
       rw [FOL.ArityToTuple.def_fromIndex t] at a_1
       . exact a_1
-      . exact a_4
+      . exact a_2
 
     | s a b p sq ih =>
       intro t
-      simp only [FOL.Query.RealizeDom.def, FOL.BoundedQuery.RealizeDom.def,
-        FOL.BoundedQuery.RealizeValidDom.def, ra_to_fol_query.isWellTyped, ra_to_fol_query_schema,
-        IsEmpty.forall_iff, DatabaseInstance.default_ran_sub_domain, and_self, and_true, and_imp,
-        RA.Query.isWellTyped.s_def, ra_to_fol_query, FOL.outVar.def,
-        FOL.BoundedQuery.Realize.tEq_def, FOL.Term.realizeSome.def,
+      simp only [RA.Query.isWellTyped.s_def, ra_to_fol_query, FOL.outVar.def,
+        FOL.Query.RealizeDom.def, FOL.BoundedQuery.Realize.tEq_def, FOL.Term.realizeSome.def,
         FirstOrder.Language.Term.realize_var, Sum.elim_inl, FOL.BoundedQuery.schema.tEq_def,
-        RA.Query.evaluateT.s_def, selectionT, ne_eq, ite_true, Set.mem_setOf_eq, implies_true,
-        true_and, forall_const] at ⊢ h
-      intro a_4 a_5 a_6 a_7 a_8 a_9 a_10
-      simp_all only [FOL.Query.RealizeDom.def, FOL.BoundedQuery.RealizeDom.def,
-        FOL.BoundedQuery.RealizeValidDom.def, IsEmpty.forall_iff,
-        DatabaseInstance.default_ran_sub_domain, and_self, and_true, and_imp, forall_const,
-        implies_true, true_and]
+        RA.Query.evaluateT.s_def, selectionT, ne_eq, ite_true, Set.mem_setOf_eq, and_imp] at ⊢ h
+      intro a_4 a_5 a_6 a_7 a_8
+      simp_all only [FOL.Query.RealizeDom.def, and_imp, forall_const, true_and]
       exact a_7
 
     | p rs sq ih =>
       intro t
-      simp only [FOL.Query.RealizeDom.def, FOL.BoundedQuery.RealizeDom.def,
-        FOL.BoundedQuery.RealizeValidDom.def, ra_to_fol_query.isWellTyped, ra_to_fol_query_schema,
-        IsEmpty.forall_iff, DatabaseInstance.default_ran_sub_domain, and_self, and_true, and_imp,
-        RA.Query.isWellTyped.p_def, ra_to_fol_query, projectQuery.def, Nat.add_zero,
-        FOL.BoundedQuery.schema.exs_def, FOL.BoundedQuery.relabel_schema, Finset.mem_pimage,
-        Part.mem_ofOption, Option.mem_def, Sum.getLeft?_eq_some_iff, forall_exists_index,
-        Finset.coe_pimage, RA.Query.evaluateT.p_def, projectionT, Set.mem_setOf_eq, forall_const,
-        implies_true] at ⊢ h
-      intro a_2 a_3 a_4 a_5
+      simp only [RA.Query.isWellTyped.p_def, ra_to_fol_query, projectQuery.def, Nat.add_zero,
+        FOL.Query.RealizeDom.def, FOL.BoundedQuery.schema.exs_def, FOL.BoundedQuery.relabel_schema,
+        Finset.coe_pimage, RA.Query.evaluateT.p_def, projectionT, Set.mem_setOf_eq, and_imp] at ⊢ h
+      intro a_2 a_3
       obtain ⟨left, right⟩ := h
-      use t
-      simp_all only [FOL.Query.RealizeDom.def, FOL.BoundedQuery.RealizeDom.def, FOL.BoundedQuery.RealizeValidDom.def,
-        ra_to_fol_query.isWellTyped, ra_to_fol_query_schema, IsEmpty.forall_iff,
-        DatabaseInstance.default_ran_sub_domain, and_self, and_true, and_imp, forall_const, implies_true, true_and]
+      have h_rs : ↑rs ⊆ t.Dom := by sorry
+      use t.restrict h_rs
+      simp_all only [FOL.Query.RealizeDom.def, ra_to_fol_query.isWellTyped, ra_to_fol_query_schema, and_imp,
+        forall_const]
       apply And.intro
-      · apply ih
-        . sorry
-        . sorry
-        . sorry
-        . sorry
-      · intro a a_1
-        sorry
+      · sorry
+      · intro a
+        apply And.intro
+        · intro a_1
+          sorry
+        · intro a_1
+          sorry
 
     | j q₁ q₂ ih₁ ih₂ =>
       intro t
-      simp only [FOL.Query.RealizeDom.def, FOL.BoundedQuery.RealizeDom.def,
-        FOL.BoundedQuery.RealizeValidDom.def, ra_to_fol_query.isWellTyped, ra_to_fol_query_schema,
-        IsEmpty.forall_iff, DatabaseInstance.default_ran_sub_domain, and_self, and_true, and_imp,
-        RA.Query.isWellTyped.j_def, ra_to_fol_query, FOL.BoundedQuery.Realize.and_def,
-        FOL.BoundedQuery.schema.and_def, Finset.mem_union, Finset.coe_union, RA.Query.evaluateT.j_def,
-        joinT, PFun.mem_dom, forall_exists_index, Set.mem_union, not_or, not_exists, Set.mem_setOf_eq,
-        forall_const, implies_true] at ⊢ h
-      intro a_2 a_3 a_4 a_5 a_6
+      simp only [RA.Query.isWellTyped.j_def, ra_to_fol_query, FOL.Query.RealizeDom.def,
+        FOL.BoundedQuery.Realize.and_def, FOL.BoundedQuery.schema.and_def, Finset.coe_union,
+        RA.Query.evaluateT.j_def, joinT, PFun.mem_dom, forall_exists_index, Set.mem_union, not_or,
+        not_exists, and_imp, Set.mem_setOf_eq] at ⊢ h
+      intro a_2 a_3 a_4
       have h_dom : t.Dom = ↑(q₁.schema dbi.schema) ∪ ↑(q₂.schema dbi.schema) := by
-        simp [h] at a_6 a_4
+        simp [h] at a_4
         obtain ⟨left, right⟩ := h
-        exact Set.Subset.antisymm a_6 a_4
 
-      have z' : ↑(q₁.schema dbi.schema) ⊆ t.Dom := by simp_all
+        have z₁ := FOL.BoundedQuery.Realize.schema_sub_Dom a_2
+        have z₂ := FOL.BoundedQuery.Realize.schema_sub_Dom a_3
+        simp_all only [FOL.Query.RealizeDom.def, ra_to_fol_query.isWellTyped, ra_to_fol_query_schema, and_imp,
+          forall_const]
+
+        apply Set.Subset.antisymm a_4 (Set.union_subset z₁ z₂)
+
+      have z' : ↑(ra_to_fol_query q₁ dbi.schema).schema ⊆ t.Dom := by simp_all
       use t.restrict (z')
       apply And.intro
       . apply ih₁
         . exact h.1
-        . sorry
+        . apply And.intro
+          . exact FOL.BoundedQuery.Realize.tuple_restrict2 (by simp [h.1]) z' a_2
+          . simp_all
+            simp [PFun.Dom, Part.dom_iff_mem, z', Set.subset_def]
+            aesop
 
-      . have z' : ↑(q₂.schema dbi.schema) ⊆ t.Dom := by simp_all
+      . have z' : ↑(ra_to_fol_query q₂ dbi.schema).schema ⊆ t.Dom := by simp_all
         use t.restrict (z')
         apply And.intro
         . apply ih₂
           . exact h.2
-          . sorry
+          . apply And.intro
+            . exact FOL.BoundedQuery.Realize.tuple_restrict2 (by simp [h.2]) z' a_3
+            . simp_all
+              simp [PFun.Dom, Part.dom_iff_mem, z', Set.subset_def]
+              aesop
 
         . intro a
           simp only [PFun.mem_restrict, Finset.mem_coe, and_imp, not_and]
@@ -131,35 +124,162 @@ theorem ra_to_fol_evalT.reverse {raQ dbi} [struc : FOL.folStruc dbi] (h : RA.Que
 
     | r => sorry
 
+theorem ra_to_fol_evalT.rf {raQ dbi} [struc : FOL.folStruc dbi] (h : RA.Query.isWellTyped dbi.schema raQ) :
+  ∀t, t ∈ RA.Query.evaluateT dbi raQ → (ra_to_fol_query raQ dbi.schema).RealizeDom dbi t := by
+    induction raQ with
+    | R rn =>
+      intro t h_RA_eval
+      apply
+        FOL.Query.Realize.imp_RealizeDom_if_t_Dom_sub_schema
+          (ra_to_fol_query (.R rn) dbi.schema)
+          (by simp_all [RA.Query.evaluate.validSchema (.R rn) h t h_RA_eval])
+
+      simp only [ra_to_fol_query]
+      simp_all only [RA.Query.isWellTyped.R_def, RA.Query.evaluateT.R_def,
+        FOL.BoundedQuery.Realize.R_def, Function.comp_apply, FOL.outVar.def,
+        FOL.Term.realizeSome.def, FirstOrder.Language.Term.realize_var, Sum.elim_inl,
+        RelationSchema.fromIndex_Dom, implies_true, FOL.BoundedQuery.toFormula_rel,
+        FirstOrder.Language.BoundedFormula.realize_rel, FOL.folStruc_apply_RelMap, true_and]
+
+      rw [FOL.ArityToTuple.def_fromIndex t]
+      . exact h_RA_eval
+      . simp [RelationInstance.validSchema.def h_RA_eval]
+
+    | s a b p sq ih =>
+      intro t h_RA_eval
+      apply
+        FOL.Query.Realize.imp_RealizeDom_if_t_Dom_sub_schema
+          (ra_to_fol_query (.s a b p sq) dbi.schema)
+          (by simp_all [RA.Query.evaluate.validSchema (.s a b p sq) h t h_RA_eval])
+
+      simp only [ra_to_fol_query]
+      simp_all only [RA.Query.isWellTyped.s_def, RA.Query.evaluateT.s_def, selectionT, ne_eq,
+        ite_true, Set.mem_setOf_eq, FOL.outVar.def, FOL.BoundedQuery.Realize.tEq_def,
+        FOL.Term.realizeSome.def, FirstOrder.Language.Term.realize_var, Sum.elim_inl,
+        and_self_left, true_and, forall_const]
+      simp_all only [FOL.Query.RealizeDom.def, ra_to_fol_query.isWellTyped, ra_to_fol_query_schema, true_and]
+      obtain ⟨left, right⟩ := h
+      obtain ⟨left_1, right_1⟩ := h_RA_eval
+      obtain ⟨left_2, right⟩ := right
+      apply And.intro
+      · have z : ∀x, x ∈ sq.schema dbi.schema ↔ (t x).Dom := by
+          simp [(RA.Query.evaluate dbi sq left).validSchema t left_1, RA.Query.evaluate, Part.dom_iff_mem, ← PFun.mem_dom]
+        simp_all only
+      · exact right_1
+
+    | p rs sq ih =>
+      intro t h_RA_eval
+      have t_Dom : t.Dom = rs := by
+        exact RA.Query.evaluate.validSchema (.p rs sq) h t h_RA_eval
+      apply
+        FOL.Query.Realize.imp_RealizeDom_if_t_Dom_sub_schema
+          (ra_to_fol_query (.p rs sq) dbi.schema)
+          (by simp_all)
+
+      simp only [ra_to_fol_query]
+      simp_all only [RA.Query.isWellTyped.p_def, RA.Query.evaluateT.p_def, projectionT,
+        Set.mem_setOf_eq, forall_const]
+      simp_all only [projectQuery.def, Nat.add_zero]
+      simp_all only [FOL.Query.RealizeDom.def, ra_to_fol_query.isWellTyped, ra_to_fol_query_schema]
+      obtain ⟨left, right⟩ := h
+      obtain ⟨w, h⟩ := h_RA_eval
+      obtain ⟨hw, right_1⟩ := h
+
+      have z := (ih w hw)
+      have w_Dom : w.Dom = sq.schema dbi.schema := by
+        exact RA.Query.evaluate.validSchema sq left w hw
+
+      sorry
+
+    | j q₁ q₂ ih₁ ih₂ =>
+      intro t h_RA_eval
+      have t_Dom : t.Dom = q₁.schema dbi.schema ∪ q₂.schema dbi.schema := by
+        exact RA.Query.evaluate.validSchema (.j q₁ q₂) h t h_RA_eval
+
+      apply
+        FOL.Query.Realize.imp_RealizeDom_if_t_Dom_sub_schema
+          (ra_to_fol_query (.j q₁ q₂) dbi.schema)
+          (by simp_all)
+
+      simp only [ra_to_fol_query]
+      simp_all only [RA.Query.isWellTyped.j_def, RA.Query.evaluateT.j_def, joinT, PFun.mem_dom,
+        forall_exists_index, Set.mem_union, not_or, not_exists, and_imp, Set.mem_setOf_eq,
+        FOL.BoundedQuery.Realize.and_def, forall_const]
+      simp_all only [FOL.Query.RealizeDom.def, ra_to_fol_query.isWellTyped, ra_to_fol_query_schema]
+
+      obtain ⟨left, right⟩ := h
+      obtain ⟨w₁, h⟩ := h_RA_eval
+      obtain ⟨hw₁, h⟩ := h
+      obtain ⟨w₂, h⟩ := h
+      obtain ⟨hw₂, right_1⟩ := h
+      apply And.intro
+      · have z := (ih₁ w₁ hw₁)
+        have w_Dom : w₁.Dom = q₁.schema dbi.schema := by
+          exact RA.Query.evaluate.validSchema q₁ left w₁ hw₁
+        have z' : w₁.Dom ⊆ t.Dom := by simp_all
+        apply FOL.BoundedQuery.Realize.tuple_restrict (ra_to_fol_query.isWellTyped q₁ dbi.schema left) z.1 z'
+
+        ext a v
+        simp [PFun.mem_restrict]
+        by_cases hc : a ∈ w₁.Dom
+        . simp [PFun.mem_dom] at hc
+          have ⟨y, hy⟩ := hc
+          have z'' := (right_1 a).1 y hy
+          simp_all only [Finset.coe_union, subset_refl, and_self, Set.subset_union_left, true_and]
+        . simp_all only [Finset.coe_union, subset_refl, and_self, Set.subset_union_left, Finset.mem_coe]
+          simp [← Finset.mem_coe, (Set.ext_iff.mp w_Dom.symm) a] at hc
+          apply Iff.intro
+          · intro a_1
+            exact False.elim (hc v a_1)
+          · intro a_1
+            obtain ⟨left_1, right_2⟩ := a_1
+            obtain ⟨w, h⟩ := left_1
+            exact False.elim (hc w h)
+
+
+      · have z := (ih₂ w₂ hw₂)
+        have w_Dom : w₂.Dom = q₂.schema dbi.schema := by
+          exact RA.Query.evaluate.validSchema q₂ right w₂ hw₂
+        have z' : w₂.Dom ⊆ t.Dom := by simp_all
+        apply FOL.BoundedQuery.Realize.tuple_restrict (ra_to_fol_query.isWellTyped q₂ dbi.schema right) z.1 z'
+
+        ext a v
+        simp [PFun.mem_restrict]
+        by_cases hc : a ∈ w₂.Dom
+        . simp [PFun.mem_dom] at hc
+          have ⟨y, hy⟩ := hc
+          have z'' := (right_1 a).2.1 y hy
+          simp_all only [Finset.coe_union, subset_refl, and_self, Set.subset_union_left, true_and]
+        . simp_all only [Finset.coe_union, subset_refl, and_self, Set.subset_union_left, Finset.mem_coe]
+          simp [← Finset.mem_coe, (Set.ext_iff.mp w_Dom.symm) a] at hc
+          apply Iff.intro
+          · intro a_1
+            exact False.elim (hc v a_1)
+          · intro a_1
+            obtain ⟨left_1, right_2⟩ := a_1
+            obtain ⟨w, h⟩ := left_1
+            exact False.elim (hc w h)
+
+    | r f sq ih =>
+      intro t h_RA_eval
+      apply
+        FOL.Query.Realize.imp_RealizeDom_if_t_Dom_sub_schema
+          (ra_to_fol_query (.r f sq) dbi.schema)
+          (by simp_all [RA.Query.evaluate.validSchema (.r f sq) h t h_RA_eval])
+
+      simp only [ra_to_fol_query]
+      simp_all only [FOL.Query.RealizeDom.def, ra_to_fol_query.isWellTyped, ra_to_fol_query_schema,
+        RA.Query.isWellTyped.r_def, RA.Query.evaluateT.r_def, renameT, exists_eq_right',
+        Set.mem_setOf_eq, forall_const, and_self, implies_true]
+      obtain ⟨left, right⟩ := h
+      sorry
+
 theorem ra_to_fol_evalT.mem (dbi : DatabaseInstance) [struc : FOL.folStruc dbi] (raQ : RA.Query) (h_ra_wt : raQ.isWellTyped dbi.schema):
   ∀t, t ∈ raQ.evaluateT dbi ↔ (ra_to_fol_query raQ dbi.schema).RealizeDom dbi t := by
     intro t
     apply Iff.intro
-    . intro h_RA_eval
-      apply
-        FOL.Query.RealizeDom.isWellTyped_eq_Realize
-          (ra_to_fol_query raQ dbi.schema)
-          (ra_to_fol_query.isWellTyped raQ dbi.schema h_ra_wt)
-          (by simp_all [RA.Query.evaluate.validSchema raQ h_ra_wt t h_RA_eval])
-          (RA.Query.evaluateT.dbi_domain h_ra_wt t h_RA_eval)
-
-
-      induction raQ with
-      | R rn =>
-        simp only [ra_to_fol_query]
-        simp_all only [RA.Query.isWellTyped.R_def, RA.Query.evaluateT.R_def,
-          FOL.BoundedQuery.Realize.R_def, Function.comp_apply, FOL.outVar.def,
-          FOL.Term.realizeSome.def, FirstOrder.Language.Term.realize_var, Sum.elim_inl,
-          RelationSchema.fromIndex_Dom, implies_true, FOL.BoundedQuery.toFormula_rel,
-          FirstOrder.Language.BoundedFormula.realize_rel, FOL.folStruc_apply_RelMap, true_and]
-
-        rw [FOL.ArityToTuple.def_fromIndex t]
-        . exact h_RA_eval
-        . sorry
-
-      | _ => simp_all [ra_to_fol_query, selectionT, projectionT, joinT, renameT]; sorry
-
-    . exact ra_to_fol_evalT.reverse h_ra_wt t
+    . exact ra_to_fol_evalT.rf h_ra_wt t
+    . exact ra_to_fol_evalT.fr h_ra_wt t
 
 theorem ra_to_fol_eval {dbi} [struc : FOL.folStruc dbi] (raQ : RA.Query) (h_ra_wt : raQ.isWellTyped dbi.schema) :
   raQ.evaluate dbi h_ra_wt = (ra_to_fol_query raQ dbi.schema).evaluate dbi := by
@@ -175,5 +295,5 @@ theorem ra_to_fol {dbi} [FOL.folStruc dbi] (raQ : RA.Query) (h : raQ.isWellTyped
     exact ra_to_fol_eval raQ h
 
 
-theorem fol_to_ra {dbi} [FOL.folStruc dbi] (folQ : FOL.Query) (h : folQ.isWellTyped) :
+theorem fol_to_ra {dbi} [FOL.folStruc dbi] (folQ : FOL.Query) (h : folQ.isWellTyped dbi.schema) :
   ∃raQ : RA.Query, ∃(h' : raQ.isWellTyped dbi.schema), raQ.evaluate dbi h' = folQ.evaluate dbi := by sorry
