RelationalAlgebra/FOL/Evaluate.lean
@@ -15,16 +15,15 @@ theorem realize_query_dom {t : Attribute →. Value}  {q : Query} (dbi : Databas
   t.Dom = q.schema := by
     ext a
     simp_all [PFun.mem_dom, Finset.mem_coe, Query.evaluateT]
-    obtain ⟨w, h⟩ := h_realize
-    obtain ⟨w_1, h⟩ := w
-    obtain ⟨left, right⟩ := h
+    obtain ⟨h_realize, h_t_sub_schema⟩ := h_realize
     apply Iff.intro
     . intro a_1
       obtain ⟨w, h_1⟩ := a_1
-      apply h
+      apply h_t_sub_schema
       exact (PFun.mem_dom t a).mpr (Exists.intro w h_1)
     . intro a_1
-      exact Part.dom_iff_mem.mp (left a (h (left a a_1)))
+      have left := BoundedQuery.Realize.schema_sub_Dom h_realize
+      exact Part.dom_iff_mem.mp (left a (h_t_sub_schema (left a a_1)))
 
 def Query.evaluate {q : Query} (dbi : DatabaseInstance) [folStruc dbi] :
   RelationInstance := ⟨q.schema, q.evaluateT dbi, λ _ ht ↦ realize_query_dom dbi ht⟩
